lean/Project.lean
@@ -3,8 +3,10 @@ import Project.BinarySearch.Rules
 import Project.BinarySearch.Program
 import Project.BinarySearch.Smoke
 import Project.BinarySearch.Spec
+import Project.BinarySearch.TotalProof
 import Project.BinarySearchOpt3.Program
 import Project.BinarySearchOpt3.Smoke
 import Project.BinarySearchOpt3.Equivalence
+import Project.BinarySearchOpt3.SymbolicEquivalence
 import Project.BinarySearchOpt3.Spec
 import Project.BinarySearchOpt3.TotalProof
